Add zoo_std/xtchain.

lib/zoo_std/xtchain.ml
@@ -1,0 +1,4 @@
+type 'a t =
+  { mutable xtchain_next: 'a t;
+    mutable xtchain_data: 'a;
+  }
