theories/zoo_std/xtchain.v
@@ -1,0 +1,282 @@
+From zoo Require Import
+  prelude.
+From zoo.language Require Import
+  notations.
+From zoo.diaframe Require Import
+  diaframe.
+From zoo_std Require Export
+  base
+  xtchain__types.
+From zoo_std Require Import
+  xchain.
+From zoo Require Import
+  options.
+
+Implicit Types node : location.
+Implicit Types nodes : list location.
+Implicit Types v next dst : val.
+
+Section zoo_G.
+  Context `{zoo_G : !ZooG Σ}.
+
+  Definition xtchain hdr nodes dst : iProp Σ :=
+    xchain nodes dst ∗
+    [∗ list] node ∈ nodes, node ↦ₕ hdr.
+
+  #[global] Instance xtchain_timeless hdr nodes dst :
+    Timeless (xtchain hdr nodes dst).
+  Proof.
+    apply _.
+  Qed.
+
+  Lemma xtchain_nil hdr dst :
+    ⊢ xtchain hdr [] dst.
+  Proof.
+    iSteps.
+  Qed.
+
+  Lemma xtchain_singleton hdr node dst :
+    xtchain hdr [node] dst ⊣⊢
+      node ↦ₕ hdr ∗
+      node.[xtchain_next] ↦ dst.
+  Proof.
+    rewrite /xtchain xchain_singleton. iSteps.
+  Qed.
+  Lemma xtchain_singleton_1 hdr node dst :
+    xtchain hdr [node] dst ⊢
+      node ↦ₕ hdr ∗
+      node.[xtchain_next] ↦ dst.
+  Proof.
+    rewrite xtchain_singleton //.
+  Qed.
+  Lemma xtchain_singleton_2 hdr node dst :
+    node ↦ₕ hdr ∗
+    node.[xtchain_next] ↦ dst -∗
+    xtchain hdr [node] dst.
+  Proof.
+    rewrite -xtchain_singleton. auto.
+  Qed.
+
+  Lemma xtchain_cons {hdr} nodes node nodes' dst :
+    nodes = node :: nodes' →
+    xtchain hdr nodes dst ⊣⊢
+      node ↦ₕ hdr ∗
+      node.[xtchain_next] ↦ from_option #@{location} dst (head nodes') ∗
+      xtchain hdr nodes' dst.
+  Proof.
+    intros ->.
+    rewrite /xtchain xchain_cons // big_sepL_cons. iSteps.
+  Qed.
+  Lemma xtchain_cons_1 {hdr} nodes node nodes' dst :
+    nodes = node :: nodes' →
+    xtchain hdr nodes dst ⊢
+      node ↦ₕ hdr ∗
+      node.[xtchain_next] ↦ from_option #@{location} dst (head nodes') ∗
+      xtchain hdr nodes' dst.
+  Proof.
+    intros. rewrite xtchain_cons //.
+  Qed.
+  Lemma xtchain_cons_2 hdr node nodes dst :
+    node ↦ₕ hdr ∗
+    node.[xtchain_next] ↦ from_option #@{location} dst (head nodes) -∗
+    xtchain hdr nodes dst -∗
+    xtchain hdr (node :: nodes) dst.
+  Proof.
+    rewrite (xtchain_cons (node :: nodes)) //. iSteps.
+  Qed.
+
+  Lemma xtchain_app {hdr} nodes nodes1 nodes2 dst :
+    nodes = nodes1 ++ nodes2 →
+    xtchain hdr nodes dst ⊣⊢
+      xtchain hdr nodes1 (from_option #@{location} dst (head nodes2)) ∗
+      xtchain hdr nodes2 dst.
+  Proof.
+    intros ->.
+    rewrite /xtchain xchain_app // big_sepL_app. iSteps.
+  Qed.
+  Lemma xtchain_app_1 {hdr} nodes nodes1 nodes2 dst :
+    nodes = nodes1 ++ nodes2 →
+    xtchain hdr nodes dst ⊢
+      xtchain hdr nodes1 (from_option #@{location} dst (head nodes2)) ∗
+      xtchain hdr nodes2 dst.
+  Proof.
+    intros. rewrite xtchain_app //.
+  Qed.
+  Lemma xtchain_app_2 hdr nodes1 nodes2 dst :
+    xtchain hdr nodes1 (from_option #@{location} dst (head nodes2)) -∗
+    xtchain hdr nodes2 dst -∗
+    xtchain hdr (nodes1 ++ nodes2) dst.
+  Proof.
+    rewrite (xtchain_app (nodes1 ++ nodes2)) //. iSteps.
+  Qed.
+
+  Lemma xtchain_snoc {hdr} nodes nodes' node dst :
+    nodes = nodes' ++ [node] →
+    xtchain hdr nodes dst ⊣⊢
+      xtchain hdr nodes' #node ∗
+      node ↦ₕ hdr ∗
+      node.[xtchain_next] ↦ dst.
+  Proof.
+    intros ->.
+    rewrite /xtchain xchain_snoc // big_sepL_snoc. iSteps.
+  Qed.
+  Lemma xtchain_snoc_1 {hdr} nodes nodes' node dst :
+    nodes = nodes' ++ [node] →
+    xtchain hdr nodes dst ⊢
+      xtchain hdr nodes' #node ∗
+      node ↦ₕ hdr ∗
+      node.[xtchain_next] ↦ dst.
+  Proof.
+    intros. rewrite xtchain_snoc //.
+  Qed.
+  Lemma xtchain_snoc_2 hdr nodes node dst :
+    xtchain hdr nodes #node -∗
+    node ↦ₕ hdr -∗
+    node.[xtchain_next] ↦ dst -∗
+    xtchain hdr (nodes ++ [node]) dst.
+  Proof.
+    rewrite (xtchain_snoc (nodes ++ [node])) //. iSteps.
+  Qed.
+
+  Lemma xtchain_lookup {hdr nodes} i node dst :
+    nodes !! i = Some node →
+    xtchain hdr nodes dst ⊣⊢
+      xtchain hdr (take i nodes) #node ∗
+      node ↦ₕ hdr ∗
+      node.[xtchain_next] ↦ from_option #@{location} dst (nodes !! S i) ∗
+      xtchain hdr (drop (S i) nodes) dst.
+  Proof.
+    intros.
+    rewrite /xtchain xchain_lookup //.
+    rewrite -{4}(take_drop_middle nodes i node) // big_sepL_app.
+    iSteps.
+  Qed.
+  Lemma xtchain_lookup_1 {hdr nodes} i node dst :
+    nodes !! i = Some node →
+    xtchain hdr nodes dst ⊢
+      xtchain hdr (take i nodes) #node ∗
+      node ↦ₕ hdr ∗
+      node.[xtchain_next] ↦ from_option #@{location} dst (nodes !! S i) ∗
+      xtchain hdr (drop (S i) nodes) dst.
+  Proof.
+    intros. rewrite xtchain_lookup //.
+  Qed.
+  Lemma xtchain_lookup_2 {hdr nodes} i node next dst :
+    nodes !! i = Some node →
+    next = from_option #@{location} dst (nodes !! S i) →
+    xtchain hdr (take i nodes) #node -∗
+    node ↦ₕ hdr -∗
+    node.[xtchain_next] ↦ next -∗
+    xtchain hdr (drop (S i) nodes) dst -∗
+    xtchain hdr nodes dst.
+  Proof.
+    intros. rewrite (@xtchain_lookup _ nodes) //. iSteps.
+  Qed.
+
+  Lemma xtchain_lookup_acc {hdr nodes} i node dst :
+    nodes !! i = Some node →
+    xtchain hdr nodes dst ⊢
+      node ↦ₕ hdr ∗
+      node.[xtchain_next] ↦ from_option #@{location} dst (nodes !! S i) ∗
+      ( node.[xtchain_next] ↦ from_option #@{location} dst (nodes !! S i) -∗
+        xtchain hdr nodes dst
+      ).
+  Proof.
+    intros. rewrite xtchain_lookup //. iSteps.
+  Qed.
+
+  Lemma xtchain_lookup_header {hdr nodes} i node dst :
+    nodes !! i = Some node →
+    xtchain hdr nodes dst ⊢
+    node ↦ₕ hdr.
+  Proof.
+    intros. rewrite xtchain_lookup //. iSteps.
+  Qed.
+
+  Lemma xtchain_exclusive hdr nodes dst1 dst2 :
+    0 < length nodes →
+    xtchain hdr nodes dst1 -∗
+    xtchain hdr nodes dst2 -∗
+    False.
+  Proof.
+    iIntros "% (H1 & _) (H2 & _)".
+    iApply (xchain_exclusive with "H1 H2"); first done.
+  Qed.
+
+  Lemma xtchain_NoDup hdr nodes dst :
+    xtchain hdr nodes dst ⊢
+    ⌜NoDup nodes⌝.
+  Proof.
+    iIntros "(H & _)".
+    iApply (xchain_NoDup with "H").
+  Qed.
+
+  Lemma xtchain_next_spec {hdr nodes node} nodes' dst E :
+    nodes = node :: nodes' →
+    {{{
+      xtchain hdr nodes dst
+    }}}
+      (#node).{xtchain_next} @ E
+    {{{
+      RET from_option #@{location} dst (head nodes');
+      xtchain hdr nodes dst
+    }}}.
+  Proof.
+    iIntros (->) "%Φ (H & Hheaders) HΦ".
+    wp_apply (xchain_next_spec with "H"); first done.
+    iSteps.
+  Qed.
+  Lemma xtchain_next_spec_lookup {hdr nodes} i node dst E :
+    nodes !! i = Some node →
+    {{{
+      xtchain hdr nodes dst
+    }}}
+      (#node).{xtchain_next} @ E
+    {{{
+      RET from_option #@{location} dst (nodes !! S i);
+      xtchain hdr nodes dst
+    }}}.
+  Proof.
+    iIntros "%Hlookup %Φ (H & Hheaders) HΦ".
+    wp_apply (xchain_next_spec_lookup with "H"); first done.
+    iSteps.
+  Qed.
+
+  Lemma xtchain_set_next_spec {hdr nodes node} nodes' dst v E :
+    nodes = node :: nodes' →
+    {{{
+      xtchain hdr nodes dst
+    }}}
+      (#node) <-{xtchain_next} v @ E
+    {{{
+      RET ();
+      xtchain hdr [node] v ∗
+      xtchain hdr nodes' dst
+    }}}.
+  Proof.
+    iIntros (->) "%Φ (H & Hheaders) HΦ".
+    wp_apply (xchain_set_next_spec with "H"); first done.
+    iSteps.
+  Qed.
+  Lemma xtchain_set_next_spec_lookup {hdr nodes} i node dst v E :
+    nodes !! i = Some node →
+    {{{
+      xtchain hdr nodes dst
+    }}}
+      #node <-{xtchain_next} v @ E
+    {{{
+      RET ();
+      xtchain hdr (take (S i) nodes) v ∗
+      xtchain hdr (drop (S i) nodes) dst
+    }}}.
+  Proof.
+    intros Hlookup.
+    setoid_rewrite xtchain_lookup at 1; last done.
+    iIntros "%Φ (H1 & Hheader & Hnode & H2) HΦ".
+    wp_store.
+    iDestruct (xtchain_snoc_2 with "H1 Hheader Hnode") as "H1".
+    rewrite -take_S_r //. iSteps.
+  Qed.
+End zoo_G.
+
+#[global] Opaque xtchain.
