theories/zoo_std/xtchain__types.v
@@ -1,0 +1,16 @@
+From zoo Require Import
+  prelude.
+From zoo.language Require Import
+  typeclasses
+  notations.
+From zoo Require Import
+  options.
+
+Notation "'xtchain_next'" := (
+  in_type "t" 0
+)(in custom zoo_field
+).
+Notation "'xtchain_data'" := (
+  in_type "t" 1
+)(in custom zoo_field
+).
